@prefix owl: <http://www.w3.org/2002/07/owl#> .
@prefix rdf: <http://www.w3.org/1999/02/22-rdf-syntax-ns#> .
@prefix rdfs: <http://www.w3.org/2000/01/rdf-schema#> .
@prefix skos: <http://www.w3.org/2004/02/skos/core#> .
@prefix xml: <http://www.w3.org/XML/1998/namespace> .
@prefix xsd: <http://www.w3.org/2001/XMLSchema#> .
@prefix dct: <http://purl.org/dc/terms/> .

<http://data.doremus.org/vocabulary/noise_reduction/> a skos:ConceptScheme ;
    rdfs:label "Techniques de réduction du bruit"@fr , "Noise Reduction Techniques"@en,
        "Tecniche di riduzione del rumore"@it ;
    rdfs:comment "Familles de techniques permettant de réduire les bruits de fond présents sur un enregistrement"@fr,
        "Generic groups of techniques or processes for removing noise from a signal"@en,
        "Famiglie di tecniche atte a ridurre il rumore di fondo da un segnale"@it ;
    dct:creator <http://data.doremus.org/organization/DOREMUS> ;
    dct:license <https://creativecommons.org/licenses/by/4.0/> ;
    dct:created "2018-08-06"^^xsd:date ;
    dct:modified "2018-08-22"^^xsd:date .

<http://data.doremus.org/vocabulary/noise_reduction/se_pre> a skos:Concept ;
    skos:definition """Systems working to affect the recording medium at the time of recording.
E.g. Dolby HX Pro."""@en ;
    skos:prefLabel "Single-ended pre-recording systems"@en ;
    skos:topConceptOf <http://data.doremus.org/vocabulary/noise_reduction/> .

<http://data.doremus.org/vocabulary/noise_reduction/se_hiss> a skos:Concept ;
    skos:definition """Systems working to to reduce noise as it occurs, including both before and after the recording process as well as for live broadcast applications.
E.g. DNL, DNR."""@en ;
    skos:prefLabel "Single-ended hiss reduction systems"@en ;
    skos:topConceptOf <http://data.doremus.org/vocabulary/noise_reduction/> .

<http://data.doremus.org/vocabulary/noise_reduction/se_surface> a skos:Concept ;
    skos:definition """Systems applied to the playback of phonograph records to attenuate the sound of scratches, pops, and surface non-linearities.
E.g. CEDAR, SAE 5000A, TNE 7000."""@en ;
    skos:prefLabel "Single-ended surface noise reduction systems"@en ;
    skos:topConceptOf <http://data.doremus.org/vocabulary/noise_reduction/> .

<http://data.doremus.org/vocabulary/noise_reduction/de> a skos:Concept ;
    skos:definition """Systems having a pre-emphasis process applied during recording and then a de-emphasis process applied at playback.
E.g. Dolby A, Dolby SR, Dolby NR, Dolby B, Dolby C, Dolby S, dbx Professional, dbx Type I, dbx Type II"""@en ;
    skos:prefLabel "Dual-ended systems"@en ;
    skos:topConceptOf <http://data.doremus.org/vocabulary/noise_reduction/> .
